Horner_Eval.thy
@@ -1,0 +1,106 @@
+theory Horner_Eval
+imports "Intervals"
+begin
+
+(* Function and lemmas for evaluating polynomials via the horner scheme.
+   Because interval multiplication is not distributive, interval polynomials
+   expressed as a sum of monomials are not equivalent to their respective horner form.
+   The functions and lemmas in this theory can be used to express interval
+   polynomials in horner form and prove facts about them. *)
+fun horner_eval'
+where "horner_eval' f x v 0 = v"
+    | "horner_eval' f x v (Suc i) = horner_eval' f x (f i + x * v) i"
+    
+fun horner_eval
+where "horner_eval f x n = horner_eval' f x 0 n"
+
+lemmas [simp del] = horner_eval.simps
+
+lemma horner_eval_cong:
+assumes "\<And>i. i < n \<Longrightarrow> f i = g i"
+assumes "x = y"
+assumes "n = m"
+shows "horner_eval f x n = horner_eval g y m"
+proof-
+  {
+    fix v have "horner_eval' f x v n = horner_eval' g x v n"
+      using assms(1) by (induction n arbitrary: v, simp_all)
+  }
+  thus ?thesis
+    by (simp add: assms(2,3) horner_eval.simps)
+qed
+    
+lemma horner_eval_eq_setsum:
+fixes x::"'a::linordered_idom"
+shows "horner_eval f x n = (\<Sum>i<n. f i * x^i)"
+proof-
+  {
+    fix v have "horner_eval' f x v n = (\<Sum>i<n. f i * x^i) + v*x^n"
+      by (induction n arbitrary: v, simp_all add: distrib_left mult.commute)
+  }
+  thus ?thesis by (simp add: horner_eval.simps)
+qed
+
+lemma horner_eval_Suc[simp]:
+fixes x::"'a::linordered_idom"
+shows "horner_eval f x (Suc n) = horner_eval f x n + (f n) * x^n"
+unfolding horner_eval_eq_setsum
+by simp
+
+lemma horner_eval_Suc'[simp]:
+fixes x::"'a::{comm_monoid_add, times}"
+shows "horner_eval f x (Suc n) = f 0 + x * (horner_eval (\<lambda>i. f (Suc i)) x n)"
+proof-
+  {
+    fix v have "horner_eval' f x v (Suc n) = f 0 + x * horner_eval' (\<lambda>i. f (Suc i)) x v n"
+    by (induction n arbitrary: v, simp_all)
+  }
+  thus ?thesis by (simp add: horner_eval.simps)
+qed
+
+lemma horner_eval_0[simp]:
+shows "horner_eval f x 0 = 0"
+by (simp add: horner_eval.simps)
+
+lemma horner_eval_interval:
+fixes x::"'a::linordered_idom"
+assumes "\<And>i. i < n \<Longrightarrow> f i \<in> set_of (g i)"
+assumes "x \<in> set_of I"
+shows "horner_eval f x n \<in> set_of (horner_eval g I n)"
+proof-
+  {
+    fix v::'a and V::"'a interval"
+    assume "v \<in> set_of V"
+    hence "horner_eval' f x v n \<in> set_of (horner_eval' g I V n)"
+      using assms
+      apply(induction n arbitrary: v V)
+      apply(simp)
+      proof(goals Suc)
+        case (Suc n v V)
+        show ?case
+          apply(simp, rule Suc(1)[OF set_of_add_mono[OF _ set_of_mult_mono]])
+          using Suc(2,3,4)
+          by (simp_all)
+      qed
+  }
+  thus ?thesis by (simp add: horner_eval.simps zero_interval_def)
+qed
+
+lemma nonempty_horner_eval:
+fixes I::"'a::linordered_idom interval"
+assumes "nonempty I"
+assumes "\<And>i. i < n \<Longrightarrow> nonempty (f i)"
+shows "nonempty (horner_eval f I n)"
+using assms
+by (induction n arbitrary: f, simp_all add: nonempty_add zero_interval_def)
+
+lemma horner_eval_interval_subset:
+fixes I::"real interval"
+assumes "nonempty I"
+assumes "set_of I \<subseteq> set_of J"
+assumes "\<And>i. i < n \<Longrightarrow> nonempty (f i)"
+shows "set_of (horner_eval f I n) \<subseteq> set_of (horner_eval f J n)"
+using assms
+by (induction n arbitrary: f, simp_all add: set_of_add_inc_right set_of_mul_inc nonempty_horner_eval)
+
+end
